Adding the function belongs

Proof.fst
@@ -38,10 +38,10 @@ val alphabet : list english_letters
 let alphabet = [A;B;C;D;E;F;G;H;I;J;K;M;N;O;P;Q;R;S;T;U;V;W;X;Y;Z]
   
 val text : list english_letters
-let text = [E;A;A;A;X;A;B;X;A;A;X;B;A;X;B;A;A;A;B;A;B;B]
+let text = [A;B;B;A;X;A;B;X;A;A;X;B;A;X;B;A;A;A;B;A;B;B]
 
 val pattern : list english_letters
-let pattern = [E;A;A;A;X;E;C;F;C]
+let pattern = [B;A;X;A;B]
 
 val alphabet_length : (i:nat{i > 0})
 let alphabet_length = length alphabet
@@ -108,154 +108,280 @@ let length_tail_is_last_index (#a:eqtype) (l:list a)
           (ensures length l = 1 + length (tl l))
   = ()
 
-let mem_index_range_index_is_item (#a:eqtype) (l:list a)
-  : Lemma (requires length l <= 7) //from 8 it doesn't work
-          (ensures forall (item:a).
-          (let i = item_index item l (length l) in
-           i <> -1 && i < length l ==> index l i = item))
-  = ()
+// let mem_index_range_index_is_item (#a:eqtype) (l:list a)
+//   : Lemma (requires length l <= 4) //from 8 it doesn't work
+//           (ensures forall (item:a).
+//           (let i = item_index item l (length l) in
+//            i <> -1 && i < length l ==> index l i = item))
+//   = ()
 
-let item_not_found_returns_minusone_specific_element (#a:eqtype) (l:list a)
-  : Lemma (requires length l <= 6) //from 7 it doesn't work
-          (ensures forall (item:a). item_index item l (length l) = -1 ==> (forall (i:nat{i < length l}). index l i <> item))
-  = ()
+// let item_not_found_returns_minusone_specific_element (#a:eqtype) (l:list a)
+//   : Lemma (requires length l <= 6) //from 7 it doesn't work
+//           (ensures forall (item:a). item_index item l (length l) = -1 ==> (forall (i:nat{i < length l}). index l i <> item))
+//   = ()
 
-let one_index_not_item (#a:eqtype) (item:a) (l:list a) (i:nat{i < length l})
-  : Type
-  = index l i <> item
+// let one_index_not_item (#a:eqtype) (item:a) (l:list a) (i:nat{i < length l})
+//   : Type
+//   = index l i <> item
 
-let item_not_found_returns_minusone_one_index (#a:eqtype) (item:a) (l:list a) (i:nat{i < length l})
-  : Lemma (requires item_index item l (length l) = -1)
-          (ensures one_index_not_item item l ((length l) - 1))
-  = ()
+// let item_not_found_returns_minusone_one_index (#a:eqtype) (item:a) (l:list a) (i:nat{i < length l})
+//   : Lemma (requires item_index item l (length l) = -1)
+//           (ensures one_index_not_item item l ((length l) - 1))
+//   = ()
 
-let rec item_not_found_item_not_found_less_indexes (#a:eqtype) (l:list a)
-  : Lemma (ensures forall (item:a). item_index item l (length l) = -1 ==> (forall (i:nat{i < length l}). item_index item l i = -1))
-  = match l with
-    | [] -> ()
-    | hd :: tl -> item_not_found_item_not_found_less_indexes tl
+// let rec item_not_found_item_not_found_less_indexes (#a:eqtype) (l:list a)
+//   : Lemma (ensures forall (item:a). item_index item l (length l) = -1 ==> (forall (i:nat{i < length l}). item_index item l i = -1))
+//   = match l with
+//     | [] -> ()
+//     | hd :: tl -> item_not_found_item_not_found_less_indexes tl
 
-let rec item_not_found_returns_minusone (#a:eqtype) (l:list a)
-  : Lemma (ensures forall (item:a). item_index item l (length l) = -1 ==> (forall (i:nat{i < length l}). one_index_not_item i))
-  = match l with
-    | [] -> ()
-    | hd :: tl -> admit(item_not_found_returns_minusone tl);
-                  item_not_found_returns_minusone_one_index l
+// let rec item_not_found_returns_minusone (#a:eqtype) (l:list a)
+//   : Lemma (ensures forall (item:a). item_index item l (length l) = -1 ==> (forall (i:nat{i < length l}). one_index_not_item i))
+//   = match l with
+//     | [] -> ()
+//     | hd :: tl -> admit(item_not_found_returns_minusone tl);
+//                   item_not_found_returns_minusone_one_index l
 
-let item_found_returns_nat (#a:eqtype) (l:list a)
-  : Lemma (ensures forall (item:a). 
-          (let i = item_index item l (length l) in
-           i <> -1 ==> i >= 0))
-  = ()
+// let item_found_returns_nat (#a:eqtype) (l:list a)
+//   : Lemma (ensures forall (item:a). 
+//           (let i = item_index item l (length l) in
+//            i <> -1 ==> i >= 0))
+//   = ()
 
-let rec item_found_returns_index (#a:eqtype) (l:list a)
-  : Lemma (ensures forall (item:a). 
-          (let i = item_index item l (length l) in
-           i <> -1 && i < length l ==> index l i = item))
-  = match l with
-    | [] -> ()
-    | hd :: tl -> item_found_returns_index tl
+// let rec item_found_returns_index (#a:eqtype) (l:list a)
+//   : Lemma (ensures forall (item:a). 
+//           (let i = item_index item l (length l) in
+//            i <> -1 && i < length l ==> index l i = item))
+//   = match l with
+//     | [] -> ()
+//     | hd :: tl -> item_found_returns_index tl
 
 //good suffix part
-val first_characters (l:list english_letters) (j:nat{j >= 0}) : list english_letters
-let rec first_characters l j =
-    match l with
-        | [] -> []
-        | hd :: tl -> if j > 0 
-                      then hd :: first_characters tl (j - 1)
-                      else first_characters tl j
-                    
-val last_characters (l:list english_letters) (dim:nat) (i:nat) (j:nat{j >= 0}) : list english_letters
-let rec last_characters l dim i j =
-    match l with
-        | [] -> []
-        | hd::tl -> if i >= dim - j
-                    then hd :: last_characters tl dim (i + 1) j
-                    else last_characters tl dim (i + 1) j
+val first_characters (l:list english_letters) (i:nat{i <= length l}) : list english_letters
+let rec first_characters l i =
+    match i with 
+    | 0 -> []
+    | _ -> (index l 0) :: (first_characters (tail l) (i - 1)) 
+           
+let first_characters_zero_is_empty_list (l:list english_letters)
+  : Lemma (ensures first_characters l 0 = [])
+  = ()
 
-val compare_frontier (l:list english_letters) (dim:nat) (i:nat) (j:nat{j >= 0}) : bool
-let compare_frontier l dim i j =
-    if first_characters l j = last_characters l dim i j && j < (length l)
+let rec length_first_characters_i_is_i (l:list english_letters) (i:nat{i <= length l})
+  : Lemma (ensures length (first_characters l i) = i)
+  = match l with
+    | [] -> ()
+    | hd :: tl -> match i with 
+                  | 0 -> ()
+                  | _ -> length_first_characters_i_is_i tl (i - 1)
+
+let rec first_characters_stores_indices_correctly_base (l:list english_letters) (i:nat{i <= length l}) (j:nat{j < i && j < length (first_characters l i)})
+  : Lemma (ensures 
+           (let l' = first_characters l i in 
+            index l' j = index l j))
+  = match l with 
+    | [] -> ()
+    | hd :: tl -> match j with 
+                  | 0 -> ()
+                  | _ -> first_characters_stores_indices_correctly_base tl (i - 1) (j - 1)
+
+let first_characters_stores_indices_correctly (l:list english_letters) (i:nat{i <= length l})
+  : Lemma (ensures forall (j:nat{j < i && j < length (first_characters l i)}).
+           (let l' = first_characters l i in 
+            index l' j = index l j))
+  = forall_intro (first_characters_stores_indices_correctly_base l i)
+
+// val last_characters (l:list english_letters) (dim:nat) (i:nat) (j:nat{j >= 0}) : list english_letters
+// let rec last_characters l dim i j =
+//     match l with
+//         | [] -> []
+//         | hd::tl -> if i >= dim - j
+//                     then hd :: last_characters tl dim (i + 1) j
+//                     else last_characters tl dim (i + 1) j
+
+val last_characters (l:list english_letters) (i:nat{i <= length l}) : list english_letters
+let rec last_characters l i =
+    match i with
+    | 0 -> []
+    | _ -> (index l ((length l) - i)) :: (last_characters (tail l) (i - 1))
+
+let last_characters_zero_is_empty_list (l:list english_letters)
+  : Lemma (ensures last_characters l 0 = [])
+  = ()
+
+let rec length_last_characters_i_is_i (l:list english_letters) (i:nat{i <= length l})
+  : Lemma (ensures length (last_characters l i) = i)
+  = match l with
+    | [] -> ()
+    | hd :: tl -> match i with 
+                  | 0 -> ()
+                  | _ -> length_last_characters_i_is_i tl (i - 1)
+
+// let lemma_aux (l:list english_letters) (i:nat{i > 0 && i <= length l}) (el:english_letters)
+//   : Lemma (ensures index l ((length l) - (i - 1))) = index (el :: l) ((length (el :: l)) - i)
+//   = admit()
+
+let rec last_characters_stores_indices_correctly_base (l:list english_letters) (i:nat{i <= length l}) (j:nat{j < i && j < length (last_characters l i)})
+  : Lemma (ensures 
+           (let l' = last_characters l i in 
+            index l' j = index l ((length l) - i)))
+  = match l with 
+    | [] -> ()
+    | hd :: tl -> match j with 
+                  | 0 -> ()
+                  | _ -> assert(last_characters l i = (index l ((length l) - i)) :: (last_characters tl (i - 1)));
+                         assert(index (last_characters l i) j = index (last_characters tl (i - 1)) (j - 1));
+                         last_characters_stores_indices_correctly_base tl (i - 1) (j - 1);
+                         assert(index (last_characters tl (i - 1)) (j - 1) = index tl ((length tl) - (i - 1)));
+                         assert(length tl = (length l) - 1);
+                         assert(index (last_characters tl (i - 1)) (j - 1) = index tl ((length l) - i));
+                         admit()
+
+val compare_frontier (l:list english_letters) (i:nat{i <= length l}) : bool
+let compare_frontier l i =
+    if first_characters l i = last_characters l i && i < (length l)
     then true
     else false
     
-val maximum (m:int) (n:int) : int
-let maximum m n =
-    if m > n 
-    then m
-    else n
+let rec compare_lists_base (l1:list english_letters) (l2:list english_letters) (i:nat{i < length l1 && i < length l2})
+  : Lemma (ensures l1 = l2 ==> (length l1 = length l2) /\ (index l1 i = index l2 i))
+  = match l1 with 
+    | [] -> ()
+    | hd1 :: tl1 -> match l2 with 
+                    | [] -> ()
+                    | hd2 :: tl2 -> match i with 
+                                    | 0 -> ()
+                                    | _ -> compare_lists_base tl1 tl2 (i - 1) 
 
-val maximum_frontier (l:list english_letters) (dim:nat) (i:nat) (j:nat{j >= 0}) : nat
-let rec maximum_frontier l dim i j =
-    match j with
-        | 0 -> 0
-        | _ -> if compare_frontier l dim i j = true
-               then j
-               else maximum_frontier l dim i (j - 1)
+let compare_lists (l1:list english_letters) (l2:list english_letters)
+  : Lemma (ensures forall (i:nat{i < length l1 && i < length l2}). l1 = l2 ==> (length l1 = length l2) && (index l1 i = index l2 i))
+  = forall_intro (compare_lists_base l1 l2)
 
-val append (#a:Type) (m:list a) (n:a) : list a
-let rec append m n = 
-    match m with
-        | [] -> n :: []
-        | hd :: tl -> hd :: (append tl n)
+let compare_frontier_true_i_less_than_length_l (l:list english_letters) (i:nat{i <= length l})
+  : Lemma (ensures compare_frontier l i ==> i < length l)
+  = ()
 
-val reverse (#a:Type) (l:list a) : list a
-let rec reverse l =
-    match l with
-        | [] -> []
-        | hd :: tl -> append (reverse tl) hd
+let not_equal_unequal (l1:list english_letters) (l2:list english_letters)
+  : Lemma (ensures ~(l1 = l2) ==> l1 <> l2)
+  = ()
 
-val create_pr (l:list english_letters) (j:nat{j >= 0}) : list int
-let rec create_pr l j =
-    match j with 
-        | 0 -> [-1]
-        | _ -> (maximum_frontier (first_characters l j) (length (first_characters l j)) 0 (length (first_characters l j))) :: (create_pr l (j - 1))
+let not_length_equal_length_unequal (l1:list english_letters) (l2:list english_letters)
+  : Lemma (ensures ~(length l1 = length l2) ==> length l1 <> length l2)
+  = ()
+
+let negation_forall_indices_is_exists_index (l1:list english_letters) (l2:list english_letters) 
+  : Lemma (ensures ~(forall (i:nat{i < length l1 && i < length l2}). index l1 i = index l2 i) ==> (exists (i:nat{i < length l1 && i < length l2}). index l1 i <> index l2 i))
+  = ()
+
+let compare_lists_false_base (l1:list english_letters) (l2:list english_letters) 
+  : Lemma (ensures ~(l1 = l2) ==> ~((length l1 = length l2) /\ (forall (i:nat{i < length l1 && i < length l2}). index l1 i = index l2 i)))
+  = compare_lists l1 l2;
+    not_equal_unequal l1 l2;
+    not_length_equal_length_unequal l1 l2;
+    negation_forall_indices_is_exists_index l1 l2;
+    admit()
+
+let compare_lists_false (l1:list english_letters) (l2:list english_letters) 
+  : Lemma (ensures l1 <> l2 ==> (length l1 <> length l2) /\ (exists (i:nat{i < length l1 && i < length l2}). index l1 i <> index l2 i))
+  = admit()
+
+let compare_frontier_true_first_characters_are_equal_with_last_characters (l:list english_letters) (i:nat{i <= length l})
+  : Lemma (ensures compare_frontier l i = true ==> first_characters l i = last_characters l i)
+  = ()
+
+let compare_first_characters_with_last_characters (l:list english_letters) (i:nat{i <= length l})
+  : Lemma (ensures forall (j:nat{j < length (first_characters l i) && j < length (last_characters l i)}).
+           (let l1 = first_characters l i in
+            let l2 = last_characters l i in 
+            l1 = l2 ==> (length l1 = length l2) && (index l1 j = index l2 j)))
+  = compare_lists (first_characters l i) (last_characters l i)
+
+let compare_frontiers_true_gives_correct_result (l:list english_letters) (i:nat{i <= length l})
+  : Lemma (ensures forall (j:nat{j < length (first_characters l i) && j < length (last_characters l i)}). 
+           (let l1 = first_characters l i in
+            let l2 = last_characters l i in 
+            compare_frontier l i = true ==> (length l1 = length l2) && (index l1 j = index l2 j) && i < length l))
+  = compare_frontier_true_i_less_than_length_l l i;
+    compare_frontier_true_first_characters_are_equal_with_last_characters l i;
+    compare_first_characters_with_last_characters l i
+
+// val maximum (m:int) (n:int) : int
+// let maximum m n =
+//     if m > n 
+//     then m
+//     else n
+
+// val maximum_frontier (l:list english_letters) (dim:nat) (i:nat) (j:nat{j <= length l}) : nat
+// let rec maximum_frontier l dim i j =
+//     match j with
+//         | 0 -> 0
+//         | _ -> if compare_frontier l dim i j = true
+//                then j
+//                else maximum_frontier l dim i (j - 1)
+
+// val append (#a:Type) (m:list a) (n:a) : list a
+// let rec append m n = 
+//     match m with
+//         | [] -> n :: []
+//         | hd :: tl -> hd :: (append tl n)
+
+// val reverse (#a:Type) (l:list a) : list a
+// let rec reverse l =
+//     match l with
+//         | [] -> []
+//         | hd :: tl -> append (reverse tl) hd
+
+// val create_pr (l:list english_letters) (j:nat{j <= length l}) : list int
+// let rec create_pr l j =
+//     match j with 
+//         | 0 -> [-1]
+//         | _ -> (maximum_frontier (first_characters l j) (length (first_characters l j)) 0 (length (first_characters l j))) :: (create_pr l (j - 1))
                
-let f : list int = reverse (create_pr pattern (length pattern))
+// let f : list int = reverse (create_pr pattern (length pattern))
 
-val give_value (f:list int) (nr:int) (i:nat{i >= 0}) : int
-let rec give_value f nr i =
-    match f with
-        | [] -> -1
-        | hd::tl -> if i = nr
-                    then hd
-                    else give_value tl nr (i + 1)
+// val give_value (f:list int) (nr:int) (i:nat{i >= 0}) : int
+// let rec give_value f nr i =
+//     match f with
+//         | [] -> -1
+//         | hd::tl -> if i = nr
+//                     then hd
+//                     else give_value tl nr (i + 1)
 
-val create_gs (f:list int) (m:nat) (i:nat{i >= 0}) : list int
-let rec create_gs f m i =
-    match i with
-        | 0 -> [(give_value f m 0) - m]
-        | _ -> ((give_value f m 0) - m + i) :: (create_gs f m (i - 1))
+// val create_gs (f:list int) (m:nat) (i:nat{i >= 0}) : list int
+// let rec create_gs f m i =
+//     match i with
+//         | 0 -> [(give_value f m 0) - m]
+//         | _ -> ((give_value f m 0) - m + i) :: (create_gs f m (i - 1))
         
-let gs : list int = reverse (create_gs f (length pattern) ((length pattern) - 1))
+// let gs : list int = reverse (create_gs f (length pattern) ((length pattern) - 1))
  
-let r : list english_letters = reverse pattern
-let g : list int = reverse (create_pr r (length r)) 
-let h : list int = reverse g
+// let r : list english_letters = reverse pattern
+// let g : list int = reverse (create_pr r (length r)) 
+// let h : list int = reverse g
 
-val change_value (l:list int) (m:int) (n:int) (i:nat{i >= 0}) : list int
-let rec change_value l m n i : Tot (list int) (decreases l) =
-    match l with
-        | [] -> []
-        | hd :: tl -> if i = m
-                      then n :: change_value tl m n (i + 1)
-                      else hd :: change_value tl m n (i + 1)
+// val change_value (l:list int) (m:int) (n:int) (i:nat{i >= 0}) : list int
+// let rec change_value l m n i : Tot (list int) (decreases l) =
+//     match l with
+//         | [] -> []
+//         | hd :: tl -> if i = m
+//                       then n :: change_value tl m n (i + 1)
+//                       else hd :: change_value tl m n (i + 1)
                       
-val update_gs (gs:list int) (h:list int) (i:int{i >= 0}) (dim:nat) : Tot (list int) (decreases i)
-let rec update_gs gs h i dim =
-    match i with
-        | 0 -> gs
-        | _ -> update_gs (change_value gs (dim - (give_value h (dim - i) 0)) (dim - i) 0) h (i - 1) dim
+// val update_gs (gs:list int) (h:list int) (i:int{i >= 0}) (dim:nat) : Tot (list int) (decreases i)
+// let rec update_gs gs h i dim =
+//     match i with
+//         | 0 -> gs
+//         | _ -> update_gs (change_value gs (dim - (give_value h (dim - i) 0)) (dim - i) 0) h (i - 1) dim
 
-let final_gs : list int = append (update_gs gs h (length pattern) (length pattern)) ((length pattern) - 1)
+// let final_gs : list int = append (update_gs gs h (length pattern) (length pattern)) ((length pattern) - 1)
 
-val give_value_letter (f:list english_letters) (nr:int) (i:nat{i >= 0}) : english_letters
-let rec give_value_letter f nr i =
-    match f with
-        | [] -> A
-        | hd::tl -> if i = nr
-                    then hd
-                    else give_value_letter tl nr (i + 1)
+// val give_value_letter (f:list english_letters) (nr:int) (i:nat{i >= 0}) : english_letters
+// let rec give_value_letter f nr i =
+//     match f with
+//         | [] -> A
+//         | hd::tl -> if i = nr
+//                     then hd
+//                     else give_value_letter tl nr (i + 1)
                     
 // val boyer_moore (k:nat) (i:nat) (m:nat) (n:nat) (t:list english_letters) (p:list english_letters) (bc:list int) (gs:list int) (alphabet:list english_letters) : Tot bool (decreases %[i;k])
 // let rec boyer_moore k i m n t p bc gs alphabet =
@@ -272,6 +398,14 @@ let rec give_value_letter f nr i =
 //                   else boyer_moore (k - 1) i m n t p bc gs alphabet
 
 //conversion functions, print and main
+let rec belongs (t:list english_letters) (p:list english_letters{length p < length t}) (i:nat{i <= length t - length p})
+  : bool 
+  = match p with
+    | [] -> true
+    | hd :: tl -> if hd = index t i 
+                  then belongs t tl (i + 1)
+                  else false
+
 let convert_to_int f =
   match f with
     | false -> 0
@@ -280,17 +414,47 @@ let convert_to_int f =
 let string_of_int_list l =
   Printf.sprintf "[%s]" (String.concat "; " (List.Tot.map (Printf.sprintf "%d") l))
 
-// let rec convert_letters_to_int (l:list english_letters) : list int =
-//   match l with
-//     | [] -> []
-//     | hd::tl -> (alphabet_character_index hd alphabet 0)::(convert_letters_to_int tl)
+let convert_character_to_int (c:english_letters) 
+  = match c with 
+    | A -> 1 
+    | B -> 2 
+    | C -> 3
+    | D -> 4
+    | E -> 5
+    | F -> 6
+    | G -> 7
+    | H -> 8
+    | I -> 9
+    | J -> 10
+    | K -> 11
+    | L -> 12
+    | M -> 13
+    | M -> 14
+    | O -> 15
+    | P -> 16
+    | Q -> 17
+    | R -> 18
+    | S -> 19
+    | T -> 20
+    | U -> 21
+    | V -> 22
+    | W -> 23
+    | X -> 24
+    | Y -> 25
+    | Z -> 26
+    | _ -> -1
+
+let rec convert_letters_to_int (l:list english_letters) : list int =
+  match l with
+    | [] -> []
+    | hd :: tl -> (convert_character_to_int hd) :: (convert_letters_to_int tl)
 
 // let convert_letter_to_int c =
 //   alphabet_character_index c alphabet 0
 
 let main() =
   let message =
-     sprintf "The result is %d\n" (item_index A pattern (length (tl pattern)))
+     sprintf "The result is %d\n" (convert_to_int (belongs text pattern 2))
   in
   print_string message
 
